theories/examples/various.v
@@ -3,7 +3,7 @@ From iris.algebra Require Import csum agree excl.
 From iris.base_logic Require Import invariants.
 From iris_ni.logrel Require Import types.
 From iris_ni.program_logic Require Import dwp heap_lang_lifting.
-From iris.proofmode Require Import tactics.
+From iris.proofmode Require Import proofmode.
 From iris.heap_lang Require Import lang proofmode.
 From iris_ni.proofmode Require Import dwp_tactics.
 From iris_ni.logrel Require Import interp.
